further simplified reln_hfs and Sign -> Sig2 reduction

theories/Shared/Libs/DLW/Utils/seteq.v
@@ -20,43 +20,48 @@
 Require Import Arith Lia List Permutation.
 
 From Undecidability.Shared.Libs.DLW.Utils 
-  Require Import php.
+  Require Import utils_tac php.
 
 From Undecidability.Shared.Libs.DLW.Wf 
   Require Import measure_ind.
 
 Set Implicit Arguments.
 
-Reserved Notation "x ≡ y" (at level 70, no associativity).
-Reserved Notation "x ⊆ y" (at level 70, no associativity).
+Local Reserved Notation "x ≡ y" (at level 70, no associativity).
+Local Reserved Notation "x ⪼ y" (at level 70, no associativity).
 
-Local Infix "~p" := (@Permutation _) (at level 70, no associativity).
+Local Notation lhd := list_has_dup.
+Local Infix "~p" := Permutation (at level 70, no associativity).
+Local Notation "⌊ l ⌋" := (length l) (at level 1, format "⌊ l ⌋").
 
-Section seteq.
+Local Infix "∈" := In (at level 70, no associativity).
+Local Infix "⊆" := incl (at level 70, no associativity).
+Local Infix "≃ₛ" := (fun l p => l ⊆ p /\ p ⊆ l) (at level 70, no associativity).
 
-  Variable X : Type.
+Section incl_extra.
 
-  (* When viewed as sets, the lists are equivalent,
-      ie closed under perm + contraction + RST *)
+  Variable (X : Type).
 
-  Inductive seteq : list X -> list X -> Prop :=
-    | seteq_nil   : nil ≡ nil
-    | seteq_skip  : forall x l m, l ≡ m -> x::l ≡ x::m
-    | seteq_swap  : forall x y l, x::y::l ≡ y::x::l
-    | seteq_dup   : forall x l, x::x::l ≡ x::l
-    | seteq_sym   : forall l m, l ≡ m -> m ≡ l 
-    | seteq_trans : forall l m k, l ≡ m -> m ≡ k -> l ≡ k
-  where "l ≡ m" := (seteq l m).
+  Implicit Type (l : list X).
 
-  Hint Constructors seteq : core.
+  Hint Resolve incl_refl incl_tl incl_cons incl_nil_l : core.
 
-  Fact perm_seteq l m : l ~p m -> l ≡ m.
-  Proof. induction 1; eauto. Qed.
+  Fact lequiv_refl l : l ≃ₛ l.
+  Proof. split; auto. Qed.
 
-  Notation "l ⊆ m" := (incl l m).
+  Fact lequiv_sym l m : l ≃ₛ m -> m ≃ₛ l.
+  Proof. simpl; tauto. Qed.
 
-  Fact incl_cons_mono (x : X) l m : l ⊆ m -> x::l ⊆ x::m.
-  Proof. intros ? ? [ -> | ]; simpl; auto. Qed.
+  Fact lequiv_trans l m k : l ≃ₛ m -> m ≃ₛ k -> l ≃ₛ k.
+  Proof. intros [] []; split; apply incl_tran with m; auto. Qed.
+
+  Fact incl_cons_simpl x l m : l ⊆ m -> x::l ⊆ x::m.
+  Proof. intros; apply incl_cons; simpl; auto. Qed.
+
+  Fact incl_tail_simpl x l : l ⊆ x::l.
+  Proof. auto. Qed.
+
+  Hint Resolve incl_cons_simpl incl_tail_simpl : core.
 
   Fact incl_swap (x y : X) l : x::y::l ⊆ y::x::l.
   Proof. intros ? [ -> | [ -> | ] ]; simpl; auto. Qed.
@@ -64,76 +69,257 @@ Section seteq.
   Fact incl_cntr (x : X) l : x::x::l ⊆ x::l.
   Proof. intros ? [ -> | [ -> | ] ]; simpl; auto. Qed.
 
-  Hint Resolve incl_refl incl_cons_mono incl_swap incl_cntr incl_tl : core.
+  Fact lequiv_swap x y l : x::y::l ≃ₛ y::x::l.
+  Proof. split; apply incl_cons; simpl; auto. Qed.
 
-  Fact seqeq_incl l m : l ≡ m -> l ⊆ m /\ m ⊆ l.
+  Fact lequiv_app_comm l m : l++m ≃ₛ m++l.
+  Proof. split; intros ?; rewrite !in_app_iff; tauto. Qed.
+
+  Fact incl_cons_l_inv l m x : x::m ⊆ l -> x ∈ l /\ m ⊆ l.
   Proof.
-    induction 1 as [ | x l m H [] | x y l | x l 
-                   | l m H []
-                   | l m k H1 IH1 H2 IH2 ]; auto.
-    split; apply incl_tran with m; tauto.
+    intros H; split.
+    + apply H; simpl; auto.
+    + apply incl_tran with (2 := H); simpl; auto.
   Qed.
 
-  Lemma list_has_dup_seteq l : list_has_dup l -> exists m, m ≡ l /\ length m < length l.
+  Hint Resolve perm_skip Permutation_cons_app : core.
+
+  Fact incl_app_r_inv l m p : m ⊆ l++p -> exists m1 m2, m ~p m1++m2 /\ m1 ⊆ l /\ m2 ⊆ p.
+  Proof.
+    induction m as [ | x m IHm ].
+    + exists nil, nil; auto.
+    + intros H; apply incl_cons_l_inv in H as (H1 & H2).
+      destruct (IHm H2) as (m1 & m2 & H3 & H4 & H5).
+      apply in_app_or in H1 as [].
+      * exists (x::m1), m2; simpl; auto.
+      * exists m1, (x::m2); simpl; auto.
+  Qed.
+  
+  Fact incl_cons_r_inv x l m : 
+         m ⊆ x::l -> exists m1 m2, m ~p m1 ++ m2 /\ Forall (eq x) m1 /\ m2 ⊆ l.
+  Proof.
+    intros H.
+    apply (@incl_app_r_inv (x::nil) _ l) in H as (m1 & m2 & H1 & H2 & H3).
+    exists m1, m2; msplit 2; auto.
+    rewrite Forall_forall.
+    intros a Ha; apply H2 in Ha; destruct Ha as [ | [] ]; auto.
+  Qed.
+
+  Fact incl_right_cons_choose x l m : m ⊆ x::l -> x ∈ m \/ m ⊆ l.
+  Proof.
+    intros H; apply incl_cons_r_inv in H
+      as ([ | y m1] & m2 & H1 & H2 & H3).
+    + right.
+      intros u H; apply H3; revert H.
+      apply Permutation_in; auto.
+    + left.
+      apply Permutation_in with (1 := Permutation_sym H1).
+      rewrite Forall_forall in H2.
+      rewrite (H2 y); left; auto.
+  Qed.
+
+  Fact incl_left_right_cons x l y m : 
+          x::l ⊆ y::m  -> y = x /\ y ∈ l 
+                       \/ y = x /\ l ⊆ m
+                       \/ x ∈ m /\ l ⊆ y::m.
+  Proof.
+    intros H; apply incl_cons_l_inv in H
+      as [ [|] H2 ]; auto.
+    apply incl_right_cons_choose in H2; tauto.
+  Qed.
+
+  Fact perm_incl_left m1 m2 l: m1 ~p m2 -> m2 ⊆ l -> m1 ⊆ l.
+  Proof. intros H1 H2 ? H; apply H2; revert H; apply Permutation_in; auto. Qed.
+
+  Fact perm_incl_right m l1 l2: l1 ~p l2 -> m ⊆ l1 -> m ⊆ l2.
+  Proof. intros H1 H2 ? ?; apply Permutation_in with (1 := H1), H2; auto. Qed.
+  
+End incl_extra.
+
+Section seteq.
+
+  Variable X : Type.
+
+  Implicit Types l : list X.
+
+  Inductive list_contract : list X -> list X -> Prop :=
+    | lc_nil      : nil ⪼  nil
+    | lc_skip     : forall x l m, l ⪼ m -> x::l ⪼ x::m
+    | lc_swap     : forall x y l, x::y::l ⪼ y::x::l
+    | lc_cntr     : forall x l, x::x::l ⪼ x::l
+    | lc_trans    : forall l m k, l ⪼ m -> m ⪼ k -> l ⪼ k
+  where "l ⪼ m" := (list_contract l m).
+
+  Hint Constructors list_contract : core.
+
+  Fact perm_lc l m : l ~p m -> l ⪼ m.
+  Proof. induction 1; eauto. Qed.
+
+  Fact lc_length l m : l ⪼ m -> ⌊m⌋ <= ⌊l⌋.
+  Proof. induction 1; simpl; lia. Qed.
+
+  Fact lc_nil_inv_l l : nil ⪼ l -> l = nil.
+  Proof.
+    intros H; apply lc_length in H.
+    destruct l; simpl in *; auto; lia.
+  Qed.
+
+  Hint Resolve perm_swap perm_trans : core.
+
+  Fact lc_length_perm l m : l ⪼ m -> ⌊m⌋ < ⌊l⌋ \/ l ~p m.
+  Proof.
+    induction 1 as [ | ? ? ? ? [] | | 
+      | ? ? ? ? [] ? [] ]; simpl; eauto;
+      repeat match goal with
+        | H: _ ⪼ _ |- _ => apply lc_length in H
+      end; lia.
+  Qed.
+
+  Fact lc_refl l : l ⪼ l.
+  Proof. apply perm_lc; auto. Qed.
+
+  (* When viewed as sets, the lists are equivalent,
+      ie closed under perm + contraction + RST *)
+
+  Inductive list_seteq : list X -> list X -> Prop :=
+    | lseq_nil   : nil ≡ nil
+    | lseq_skip  : forall x l m, l ≡ m -> x::l ≡ x::m
+    | lseq_swap  : forall x y l, x::y::l ≡ y::x::l
+    | lseq_dup   : forall x l, x::x::l ≡ x::l
+    | lseq_sym   : forall l m, l ≡ m -> m ≡ l 
+    | lseq_trans : forall l m k, l ≡ m -> m ≡ k -> l ≡ k
+  where "l ≡ m" := (list_seteq l m).
+
+  Hint Constructors list_seteq : core.
+
+  Fact lc_lseq l m : l ⪼ m -> l ≡ m.
+  Proof. induction 1; eauto. Qed.
+
+  Hint Resolve perm_lc lc_lseq : core.
+
+  Fact perm_lseq l m : l ~p m -> l ≡ m.
+  Proof. auto. Qed.
+
+  Hint Resolve incl_refl incl_cons_simpl incl_swap incl_cntr incl_tl incl_tran : core.
+
+  Fact lseq_lequiv l m : l ≡ m -> l ≃ₛ m.
+  Proof.
+    induction 1 as [ | ? ? ? ? [] | | 
+                   | ? ? ? []
+                   | ? ? ? ? [] ? [] ]; eauto.
+  Qed.
+ 
+  Hint Resolve lseq_lequiv : core.
+
+  Fact lc_lequiv l m : l ⪼ m -> l ≃ₛ m.
+  Proof. intro; apply lseq_lequiv; auto. Qed.
+
+  Hint Resolve incl_l_nil : core.
+
+  Fact lc_nil_inv_r l : l ⪼ nil -> l = nil.
+  Proof. intros H; apply lc_lequiv in H as []; auto. Qed.
+ 
+  Hint Resolve list_has_dup_swap in_eq in_cons in_list_hd0 in_list_hd1 : core.
+
+  Notation lhd_cons_iff := list_has_dup_cons_iff.
+
+  Fact lc_lhd l m : l ⪼ m -> lhd m -> lhd l.
+  Proof.
+    induction 1 as [ | x l m H IH | | | ]; eauto.
+    rewrite !lhd_cons_iff; intros []; auto.
+    apply lc_lequiv in H as []; auto.
+  Qed.
+
+  Fact lseq_incl l m : l ≡ m -> l ⊆ m.
+  Proof. intro; apply lseq_lequiv; auto. Qed.
+
+  (* A list with a dup is contractible in a smaller one *) 
+
+  Lemma lhd_lc l : lhd l -> exists m, l ⪼ m /\ ⌊m⌋ < ⌊l⌋.
   Proof.
     induction 1 as [ l x H | l x H (m & H1 & H2) ].
-    + induction l as [ | y l IHl ].
-      * exfalso; destruct H.
-      * destruct H as [ -> | H ].
-        - exists (x::l); simpl; split; auto; lia.
-        - destruct (IHl H) as (m & H1 & H2).
-          exists (y::m); simpl in *; split; try lia.
-          apply seteq_trans with (y::x::l); auto.
-    + exists (x::m); simpl; split; auto; lia.
+    + apply in_split in H as (l1 & l2 & ->).
+      exists (l1++x::l2); split; simpl; try lia.
+      apply lc_trans with (x::x::l1++l2).
+      * apply perm_lc, perm_skip, Permutation_sym,
+              Permutation_cons_app; auto.
+      * apply lc_trans with (1 := lc_cntr _ _), perm_lc,
+              Permutation_cons_app; auto.
+    + exists (x::m); split; simpl; auto; lia.
   Qed.
 
-  (* The proof by induction on |l|+|m| for l ⊆ m and m ⊆ l
+  Hint Resolve lc_lseq : core.
 
-      Three cases:
+  Lemma lhd_lseq l : lhd l -> exists m, l ≡ m /\ ⌊m⌋ < ⌊l⌋.
+  Proof. intro H; apply lhd_lc in H as (? & ? & ?); eauto. Qed.
 
-      (1) m has dup    (2) l ~p m      (3) l has dup
+  Hint Constructors list_contract : core.
 
-      For (2) If l ~p m then it is trivial
+  Hint Resolve lc_refl lc_lhd : core.
 
-      Otherwise (1 or 3), if eg l has dup then l ≡ l' for a shorter l' 
-      we deduce l' ⊆ m and m ⊆ l' by seqeq_incl
-      and apply the induction hypothesis to (l',m)
-
-    *)
-
-  Lemma incl_seteq l m : l ⊆ m -> m ⊆ l -> l ≡ m.
+  Lemma lequiv_php_choose l m : l ≃ₛ m -> l ~p m \/ lhd l \/ lhd m.
   Proof.
-    induction on l m as IH with measure (length l + length m).
-    intros H1 H2.
-    destruct (le_lt_dec (length l) (length m)) as [ H3 | H3 ];
-      [ destruct length_le_and_incl_implies_dup_or_perm with (1 := H3)
-        as [ H4 | H4 ]; auto | ].
-    + destruct list_has_dup_seteq with (1 := H4) as (m' & H5 & H6).
-      apply seteq_trans with m'; auto.
-      apply seqeq_incl in H5; destruct H5.
-      apply IH; try lia; apply incl_tran with m; auto.
-    + apply seteq_sym, perm_seteq; auto.
-    + generalize (finite_php_dup H3 H1); intros H4.
-      destruct list_has_dup_seteq with (1 := H4) as (m' & H5 & H6).
-      apply seteq_trans with m'; auto.
-      apply seqeq_incl in H5; destruct H5.
-      apply IH; try lia; apply incl_tran with l; auto.
+    intros [ I1 I2 ].
+    destruct (le_lt_dec ⌊m⌋ ⌊l⌋) as [ H1 | H1 ].
+    + apply length_le_and_incl_implies_dup_or_perm in H1; tauto.
+    + apply finite_php_dup in H1; tauto.
   Qed.
 
-  Hint Resolve seqeq_incl incl_seteq : core.
+  (* if l and m are equivalent, either
+     1) l ~p m in which case l is contractible into m
+     2) lhd l hence l is contracted into a smaller one and recursion
+     3) lhd m hence m is contracted into a smaller one and recursion
+   *)
+
+  Hint Resolve lequiv_trans : core.
+
+  Lemma lequiv_lc l m : l ≃ₛ m -> exists c, l ⪼ c /\ m ⪼ c.
+  Proof.
+    induction on l m as IH with measure (⌊l⌋+⌊m⌋); intros H1.
+    destruct (lequiv_php_choose H1) as [ H2 | [ H2 | H2 ] ]; eauto.
+    + apply lhd_lc in H2 as (c & ? & ?).
+      destruct (IH c m) as (d & ? & ?); eauto; lia.
+    + apply lhd_lc in H2 as (c & ? & ?).
+      destruct (IH l c) as (d & ? & ?); eauto; lia.
+  Qed.
+
+  Lemma lequiv_lseq l m : l ≃ₛ m -> l ≡ m.
+  Proof. intros H; apply lequiv_lc in H as (c & []); eauto. Qed.
+
+  Hint Resolve lequiv_lseq : core.
 
   (* seteq is equivalent to bi-inclusion *)
 
-  Theorem seteq_bi_incl l m : l ≡ m <-> l ⊆ m /\ m ⊆ l.
-  Proof. split; auto; intros []; auto. Qed.
+  Theorem lseq_lequiv_iff l m : l ≡ m <-> l ≃ₛ m.
+  Proof. split; auto. Qed.
+
+  (* A nice induction principle for list bi-inclusion *)
+
+  Section lequiv_ind.
+
+    Variables (P : list X -> list X -> Prop)
+              (HP0 : P nil nil)
+              (HP1 : forall x l m, l ≃ₛ m -> P l m -> P (x::l) (x::m))
+              (HP2 : forall x y l, P (x::y::l) (y::x::l))
+              (HP3 : forall x l, P (x::x::l) (x::l))
+              (HP4 : forall l m, l ≃ₛ m -> P l m -> P m l)
+              (HP5 : forall l m k, l ≃ₛ m -> P l m -> m ≃ₛ k -> P m k -> P l k).
+
+    Theorem lequiv_ind l m : l ≃ₛ m -> P l m.
+    Proof. rewrite <- lseq_lequiv_iff; induction 1; eauto. Qed.
+
+  End lequiv_ind.
+
+  Lemma lequiv_lhd_or_contract l m : l ≃ₛ m -> lhd m \/ l ⪼  m.
+  Proof.
+    simpl; intros H.
+    destruct lequiv_lc with (1 := H) as (d & H1 & H2).
+    apply lc_length_perm in H2 as [ H2 | H2 ].
+    + apply finite_php_dup in H2; auto.
+      apply lc_lseq, lseq_lequiv in H1.
+      apply incl_tran with l; tauto.
+    + right; apply lc_trans with (1 := H1).
+      apply perm_lc, Permutation_sym; auto.
+  Qed.
 
 End seteq.
-
-Local Infix "≡" := seteq.
-Local Infix "⊆" := incl.
-
-(*
-Print seteq.
-Check seteq_bi_incl.
-Print Assumptions seteq_bi_incl.
-*)
